compose/SimSymbDrop.v
@@ -1,0 +1,165 @@
+Require Import Events.
+Require Import Values.
+Require Import AST.
+Require Import Asmregs.
+Require Import Memory.
+Require Import Globalenvs.
+Require Import Smallstep.
+Require Import CoqlibC.
+Require Import Skeleton.
+Require Import Integers.
+Require Import ASTC.
+Require Import LinkingC.
+Require Import SimSymb.
+Require Import MapsC.
+
+
+Set Implicit Arguments.
+
+Require Import SimDef SimSymb.
+Require Import SimMem.
+Require Import SimMemInj.
+
+(* Definition t': Type := ident -> bool. *)
+Definition t': Type := ident -> Prop.
+
+Inductive sim_sk (ss: t') (sk_src sk_tgt: Sk.t): Prop :=
+| sim_sk_intro
+    (KEPT: forall
+        id
+        (KEPT: ~ ss id)
+      ,
+       sk_tgt.(prog_defmap) ! id = sk_src.(prog_defmap) ! id)
+    (DROP: forall
+        id
+        (DROP: ss id)
+      ,
+        sk_tgt.(prog_defmap) ! id = None)
+    (* (SIMSK: forall *)
+    (*     id *)
+    (*   , *)
+    (*    sk_tgt.(prog_defmap) ! id = if ss id then None else sk_src.(prog_defmap) ! id) *)
+    (PUB: sk_src.(prog_public) = sk_tgt.(prog_public))
+    (MAIN: sk_src.(prog_main) = sk_tgt.(prog_main))
+.
+
+Inductive sim_skenv (sm0: SimMem.t) (ss: t') (skenv_src skenv_tgt: SkEnv.t): Prop :=
+| sim_skenv_intro
+    (SIMSYMB1: forall
+        id blk_src blk_tgt delta
+        (SIMVAL: SimMem.sim_val sm0 (Vptr blk_src Ptrofs.zero true) (Vptr blk_tgt delta true))
+        (BLKSRC: skenv_src.(Genv.find_symbol) id = Some blk_src)
+      ,
+        <<DELTA: delta = Ptrofs.zero>> /\ <<BLKTGT: skenv_tgt.(Genv.find_symbol) id = Some blk_tgt>>
+                                          /\ <<KEPT: ~ ss id>>
+    )
+    (SIMSYMB2: forall
+        id
+        (KEPT: ~ ss id)
+        blk_src
+        (BLKSRC: skenv_src.(Genv.find_symbol) id = Some blk_src)
+      ,
+        exists blk_tgt,
+          <<BLKTGT: skenv_tgt.(Genv.find_symbol) id = Some blk_tgt>> /\
+           <<SIM: SimMem.sim_val sm0 (Vptr blk_src Ptrofs.zero true) (Vptr blk_tgt Ptrofs.zero true)>>)
+    (SIMSYMB3: forall
+        id blk_tgt
+        (BLKTGT: skenv_tgt.(Genv.find_symbol) id = Some blk_tgt)
+      ,
+        exists blk_src,
+          <<BLKSRC: skenv_src.(Genv.find_symbol) id = Some blk_src>>
+           /\ <<SIM: SimMem.sim_val sm0 (Vptr blk_src Ptrofs.zero true) (Vptr blk_tgt Ptrofs.zero true)>>
+             (* /\ <<KEPT: ss.(kept) id>> *)
+    )
+    (SIMDEF: forall
+          blk_src blk_tgt delta def_tgt
+          (SIMFPTR: sm0.(SimMem.sim_val) (Vptr blk_src Ptrofs.zero true) (Vptr blk_tgt delta true))
+          (DEFTGT: skenv_tgt.(Genv.find_def) blk_tgt = Some def_tgt)
+        ,
+          exists def_src, <<DEFSRC: skenv_src.(Genv.find_def) blk_src = Some def_src>> /\
+                          <<DELTA: delta = Ptrofs.zero>> /\
+                          <<SIM: sim_def def_src def_tgt>>)
+.
+
+Global Program Definition link_ss (ss0 ss1: t'): option t' :=
+  (* Some (fun id => orb (ss0 id) (ss1 id)) *)
+  Some (ss0 \1/ ss1)
+.
+
+Global Program Instance Linker_t: Linker t' := {|
+  link := link_ss;
+  linkorder (ss0 ss1: t') := ss0 <1= ss1;
+|}.
+
+Global Program Instance sim_def_PreOrder: RelationClasses.PreOrder sim_def.
+Next Obligation.
+  admit "easy".
+Qed.
+Next Obligation.
+  admit "easy".
+Qed.
+
+
+
+Tactic Notation "u" "in" hyp(H) := repeat (autounfold with * in H; cbn in H).
+Tactic Notation "u" := repeat (autounfold with *; cbn).
+Tactic Notation "u" "in" "*" := repeat (autounfold with * in *; cbn in *).
+
+Global Program Instance SimSymbDrop: SimSymb.class SimMemInj := {
+  t := t';
+  sim_sk := sim_sk;
+  sim_skenv := sim_skenv;
+}
+.
+(* Next Obligation. *)
+(*   inv SIMSK. *)
+(*   econs; eauto. *)
+(*   ii. *)
+(*   destruct (classic (ss id)). *)
+(*   - erewrite DROP in *; eauto. ss. *)
+(*   - erewrite <- KEPT; ss. *)
+(*     esplits; eauto. *)
+(*     reflexivity. *)
+(* Qed. *)
+Next Obligation.
+  admit "See 'link_match_program' in Unusedglobproof.v.
+Note that we have one more goal (exists ss) but it is OK, as the 'link_match_program' proof already proves it.".
+Qed.
+Next Obligation.
+  admit "See 'init_meminj_preserves_globals' in Unusedglobproof.v".
+Qed.
+Next Obligation.
+  admit "The proof must exist in Unusedglobproof.v. See match_stacks_preserves_globals, match_stacks_incr".
+Qed.
+Next Obligation.
+(* THIS IS TOP *)
+  inv SIMSKENV. ss.
+  econs; eauto; ii; ss.
+  - inv LESRC.
+    destruct (classic (defs sk_src id)); cycle 1.
+    { exfalso. exploit SYMBDROP; eauto. i; des. clarify. }
+    exploit SYMBKEEP; eauto. intro KEEP; des.
+
+    exploit SIMSYMB1; eauto. { rewrite <- KEEP. ss. } i; des.
+
+    inv LETGT.
+    destruct (classic (defs sk_tgt id)); cycle 1.
+    { erewrite SYMBDROP0; ss.
+      exfalso.
+      clear - H H0 SIMSK.
+      inv SIMSK.
+      apply H0.
+      u.
+      destruct (classic (ss id)); cycle 1.
+      - erewrite KEPT; ss.
+      - !!!!!!!!!!!!!!!!! Somehow we need to know that, dropped ids are not in injection.
+    }
+      clear - SIMSK. admit "". }
+    erewrite SYMBKEEP0; ss.
+  -
+Qed.
+Next Obligation.
+  inv SIMSKENV.
+  econs; eauto.
+Qed.
+
